theories/L/AbstractMachines/Computable/Lookup.v
@@ -3,7 +3,7 @@ From Undecidability.L.Datatypes Require Import Lists.
 
 From Undecidability.L.AbstractMachines Require Import AbstractHeapMachineDef Computable.Shared.
 
-Definition lookupTime l x := (x+1) * (l*15 + 38).
+Definition lookupTime l x := (x+1) * (l*15 + 41).
 
 Instance term_lookup : computableTime' lookup (fun H _ => (5,fun alpha _ => (1,fun x _ => (lookupTime (length H) x ,tt)))).
 extract. unfold lookupTime. solverec.
