theories/L/Complexity/Reductions/Cook/FlatPR_to_BinaryPR.v
@@ -150,7 +150,7 @@ Qed.
 
 (** *extraction *)
 From Undecidability.L.Tactics Require Import LTactics GenEncode.
-From Undecidability.L.Datatypes Require Import  LProd LOptions LBool LLNat LLists.
+From Undecidability.L.Datatypes Require Import  LProd LOptions LBool.
 From Undecidability.L.Complexity Require Import PolyBounds. 
 
 (*repEl *)
